update parallel step and confluence lemmas

dsn/Lang/Util.lean
@@ -342,3 +342,50 @@ theorem List.disjoint_swap {α} [BEq α] {xs ys : List α} :
   induction xs with
   | nil => exact inter_empty_eq_empty
   | cons => sorry
+
+
+inductive ReflTrans (R : α → α → Prop) : α → α → Prop
+| refl e : ReflTrans R e e
+| step : R e e' → ReflTrans R e' e'' → ReflTrans R e e''
+
+
+inductive ReflTransLeft (R : α → α → Prop) : α → α → Prop
+| refl e : ReflTransLeft R e e
+| step : ReflTransLeft R e e' → R e' e'' → ReflTransLeft R e e''
+
+theorem ReflTransLeft.transitivity :
+  ReflTransLeft R e e' → ReflTransLeft R e' e'' → ReflTransLeft R e e''
+:= by
+  intro h0 h1
+  induction h1 with
+  | refl =>
+    exact h0
+  | step h2 h3 ih =>
+    exact step ih h3
+
+
+theorem ReflTrans.transitivity :
+  ReflTrans R e e' → ReflTrans R e' e'' → ReflTrans R e e''
+:= by
+  intro h0 h1
+  induction h0 with
+  | refl =>
+    exact h1
+  | step h2 h3 ih =>
+    exact step h2 (ih h1)
+
+theorem ReflTrans.reverse :
+  ReflTrans R e e' → ReflTransLeft R e e'
+:= by
+  intro h0
+  induction h0 with
+  | refl e =>
+    exact ReflTransLeft.refl e
+  | @step e em e' h1 h2 ih =>
+    apply ReflTransLeft.transitivity
+    {
+      apply ReflTransLeft.step
+      { exact ReflTransLeft.refl e }
+      { exact h1 }
+    }
+    { exact ih }
