dsn/Lang/Dynamic/NStepStar.lean
@@ -59,31 +59,183 @@ theorem NStepStar.iso :
   | step h1 h2 ih =>
     apply NStepStar.step (NStep.iso h1) ih
 
-theorem NStepStar.iso_inversion :
-  NStepStar (Expr.iso label body) e →
-  ∃ body' , e = (Expr.iso label body') ∧  NStepStar body body'
-:= by
-  intro h0
-  apply NStepStar.reverse at h0
+-- theorem NStepStar.iso_inversion :
+--   NStepStar (Expr.iso label body) e →
+--   ∃ body' , e = (Expr.iso label body') ∧  NStepStar body body'
+-- := by
+--   intro h0
+--   apply NStepStar.reverse at h0
 
-  induction h0 with
-  | refl =>
-    exists body
-    simp
-    apply NStepStar.refl
-  | step h1 h2 ih =>
-    have ⟨body',h3,h4⟩ := ih
-    clear ih
-    rw [h3] at h2
+--   induction h0 with
+--   | refl =>
+--     exists body
+--     simp
+--     apply NStepStar.refl
+--   | step h1 h2 ih =>
+--     have ⟨body',h3,h4⟩ := ih
+--     clear ih
+--     rw [h3] at h2
 
-    cases h2 with
-    | @iso body' body'' _ step =>
-      exists body''
-      simp
-      apply NStepStar.transitivity h4
-      apply NStepStar.step step
-      exact refl
+--     cases h2 with
+--     | @iso body' body'' _ step =>
+--       exists body''
+--       simp
+--       apply NStepStar.transitivity h4
+--       apply NStepStar.step step
+--       exact refl
 
+-- mutual
+
+--   theorem List.pattern_match_entry_subject_reduction :
+--     NRcdStep r r' →
+--     List.pattern_match_entry l p r = some m →
+--     ∃ m' , List.pattern_match_entry l p r' = some m'
+--   := by
+--     intro h0 h1
+--     cases h0 with
+--     | @head l' r e e' fresh step =>
+--       simp [List.pattern_match_entry] at h1
+--       by_cases h3 : l' = l
+--       {
+--         simp [*] at h1
+--         have ⟨m',ih⟩ := Expr.pattern_match_subject_reduction step h1
+--         exists m'
+--         simp [List.pattern_match_entry, *]
+--       }
+--       {
+--         simp [*] at h1
+--         exists m
+--         simp [List.pattern_match_entry, *]
+--       }
+
+--     | @tail l' r r' e fresh step =>
+--       simp [List.pattern_match_entry] at h1
+--       by_cases h3 : l' = l
+--       {
+--         simp [*] at h1
+--         exists m
+--         simp [List.pattern_match_entry, *]
+
+--       }
+--       {
+--         simp [*] at h1
+--         have ⟨m',ih⟩ := List.pattern_match_entry_subject_reduction step h1
+--         exists m'
+--         simp [List.pattern_match_entry, *]
+--       }
+
+
+
+--   theorem List.pattern_match_record_subject_reduction :
+--     NRcdStep r r' →
+--     List.pattern_match_record r rp = some m →
+--     ∃ m' , List.pattern_match_record r' rp = some m'
+--   := by cases rp with
+--   | nil =>
+--     intro h0 h1
+--     simp [List.pattern_match_record]
+--   | cons lp rp' =>
+--     have (l,p) := lp
+--     intro h0 h1
+--     simp [List.pattern_match_record] at h1
+--     have ⟨h2,h3⟩ := h1
+--     clear h1
+
+--     cases h4 : (List.pattern_match_entry l p r) with
+--     | some m0 =>
+--       simp [h4] at h3
+--       cases h5 : (List.pattern_match_record r rp') with
+--       | some m1 =>
+--         simp [h5] at h3
+--         have ⟨h6,h7⟩ := h3
+--         have ⟨m0',h8⟩ := List.pattern_match_entry_subject_reduction h0 h4
+--         have ⟨m1',h9⟩ := List.pattern_match_record_subject_reduction h0 h5
+--         exists (m0' ++ m1')
+--         simp [List.pattern_match_record, *]
+
+--       | none =>
+--         simp [h5] at h3
+--     | none =>
+--       simp [h4] at h3
+
+
+--   theorem Expr.pattern_match_subject_reduction :
+--     NStep arg arg' →
+--     Expr.pattern_match arg p = some m →
+--     ∃ m' , Expr.pattern_match arg' p = some m'
+--   := by cases p with
+--   | var x =>
+--     intro h0 h1
+--     exists [(x,arg')]
+--     simp [Expr.pattern_match]
+--   | iso l p' =>
+--     intro h0 h1
+--     cases h0 with
+--     | @iso e e' l' step =>
+--       simp [Expr.pattern_match] at h1
+--       have ⟨h2,h3⟩ := h1
+--       clear h1
+--       have ⟨m',ih⟩ := Expr.pattern_match_subject_reduction step h3
+--       exists m'
+--       simp [Expr.pattern_match]
+--       exact ⟨h2, ih⟩
+--     | _ =>
+--       simp [Expr.pattern_match] at h1
+--   | record ps =>
+--     intro h0 h1
+--     cases h0 with
+--     | iso =>
+--       simp [Expr.pattern_match] at h1
+--     | @record r r' step =>
+--       simp [Expr.pattern_match] at h1
+--       have ⟨m',ih⟩ := List.pattern_match_record_subject_reduction step h1
+--       exists m'
+--       simp [Expr.pattern_match]
+--       exact ih
+--     | _ =>
+--       simp [Expr.pattern_match] at h1
+-- end
+
+
+-- theorem Expr.pattern_match_subject_star_reduction :
+--   NStepStar arg arg' →
+--   ∀ {m},
+--   Expr.pattern_match arg p = some m →
+--   ∃ m' , Expr.pattern_match arg' p = some m'
+-- := by
+--   intro h0
+--   induction h0 with
+--   | refl =>
+--     intro m h1
+--     exists m
+--   | @step arg argm arg' h1 h2 ih =>
+--     intro m h3
+--     have ⟨m',h4⟩ := Expr.pattern_match_subject_reduction h1 h3
+--     apply ih h4
+
+
+-- theorem NStepStar.pattern_match_preservation :
+--   NStepStar arg arg' →
+--   ∀ {m m'},
+--   Expr.pattern_match arg p = some m →
+--   Expr.pattern_match arg' p = some m' →
+--   ∀ body, NStepStar (Expr.sub m body) (Expr.sub m' body)
+-- := by
+--   intro h0
+--   induction h0 with
+--   | @refl arg =>
+--     intro m m' h1 h2 body
+--     rw [h1] at h2
+--     simp at h2
+--     rw [← h2]
+--     apply NStepStar.refl
+--   | @step arg argm arg' h1 h2 ih =>
+--     intro m m' h3 h4 body
+--     have ⟨mm,h5⟩ := Expr.pattern_match_subject_reduction h1 h3
+--     have h6 := NStep.pattern_match_preservation h1 h3 h5 body
+--     apply NStepStar.transitivity h6
+--     apply ih h5
+--     apply h4
 
 
 theorem NStepStar.app_inversion :
@@ -91,14 +243,19 @@ theorem NStepStar.app_inversion :
   (∃ cator' arg' , e = (Expr.app cator' arg') ∧
     NStepStar cator cator' ∧ NStepStar arg arg'
   ) ∨
-  (∃ p body f m, e = Expr.sub m body ∧
+  (∃ m' body p f arg',
+    NStepStar (Expr.sub m' body) e ∧
     NStepStar cator (.function ((p,body)::f)) ∧
-    Expr.pattern_match arg p = some m
+    NStepStar arg arg' ∧
+    Expr.pattern_match arg' p = some m'
   ) ∨
-  (arg.is_value ∧ (∃ p body f, e = (.app (.function f) arg) ∧
+  (∃ f arg' p body,
+    NStepStar (.app (.function f) arg') e ∧
     NStepStar cator (.function ((p,body)::f)) ∧
-    Expr.pattern_match arg p = none
-  ))
+    NStepStar arg arg' ∧
+    arg'.is_value ∧
+    Expr.pattern_match arg' p = none
+  )
 := by
   intro h0
   have h1 := NStepStar.reverse h0
@@ -117,6 +274,7 @@ theorem NStepStar.app_inversion :
       clear h4
       rw [h5] at h3
       clear h5
+
       cases h3 with
       | @applicator cator' cator'' _ step =>
         apply Or.inl
@@ -133,15 +291,14 @@ theorem NStepStar.app_inversion :
 
       | @applicand arg' arg'' _ step =>
         apply Or.inl
-        exists cator'
-        exists arg''
+        exists cator', arg''
         simp
         apply And.intro h6
         apply NStepStar.transitivity h7
         apply NStepStar.step step
         apply NStepStar.refl
 
-      | pattern_match =>
+      | @pattern_match _ p m body f matching =>
         sorry
       | skip =>
         sorry
@@ -232,28 +389,28 @@ theorem NStepStar.record :
     { exact ih }
 
 
-theorem NStepStar.record_inversion :
-  NStepStar (.record r) e →
-  ∃ r' , e = .record r' ∧ NRcdStepStar r r'
-:= by
-  intro h0
-  apply NStepStar.reverse at h0
+-- theorem NStepStar.record_inversion :
+--   NStepStar (.record r) e →
+--   ∃ r' , e = .record r' ∧ NRcdStepStar r r'
+-- := by
+--   intro h0
+--   apply NStepStar.reverse at h0
 
-  induction h0 with
-  | refl =>
-    exists r
-    simp
-    exact NRcdStepStar.refl
-  | step h1 h2 ih =>
-    have ⟨r',h3,h4⟩ := ih
-    rw [h3] at h2
-    cases h2 with
-    | @record r' r'' step =>
-      exists r''
-      simp
-      apply NRcdStepStar.transitivity h4
-      apply NRcdStepStar.step step
-      exact NRcdStepStar.refl
+--   induction h0 with
+--   | refl =>
+--     exists r
+--     simp
+--     exact NRcdStepStar.refl
+--   | step h1 h2 ih =>
+--     have ⟨r',h3,h4⟩ := ih
+--     rw [h3] at h2
+--     cases h2 with
+--     | @record r' r'' step =>
+--       exists r''
+--       simp
+--       apply NRcdStepStar.transitivity h4
+--       apply NRcdStepStar.step step
+--       exact NRcdStepStar.refl
 
 theorem NStepStar.function_inversion :
   NStepStar (.function f) e →
@@ -358,42 +515,41 @@ theorem Joinable.app :
 
 
 
-theorem NStepStar.pattern_match :
-  Expr.pattern_match arg p = some m →
-  NStepStar cator (Expr.function ((p, body) :: f)) →
-  NStepStar (Expr.app cator arg) (Expr.sub m body)
-:= by
-  intro h0 h1
-  generalize h2 : (Expr.function ((p, body) :: f)) = cator' at h1
-  induction h1 with
-  | refl =>
-    rw [← h2]
-    apply NStepStar.step
-    { apply NStep.pattern_match ; exact h0 }
-    { exact .refl }
-  | step h3 h4 ih =>
-    specialize ih h2
-    apply NStepStar.step
-    { apply NStep.applicator ; exact h3 }
-    { exact ih }
+-- theorem NStepStar.pattern_match :
+--   Expr.pattern_match arg p = some m →
+--   NStepStar cator (Expr.function ((p, body) :: f)) →
+--   NStepStar (Expr.app cator arg) (Expr.sub m body)
+-- := by
+--   intro h0 h1
+--   generalize h2 : (Expr.function ((p, body) :: f)) = cator' at h1
+--   induction h1 with
+--   | refl =>
+--     rw [← h2]
+--     apply NStepStar.step
+--     { apply NStep.pattern_match ; exact h0 }
+--     { exact .refl }
+--   | step h3 h4 ih =>
+--     specialize ih h2
+--     apply NStepStar.step
+--     { apply NStep.applicator ; exact h3 }
+--     { exact ih }
 
-theorem Joinable.pattern_match :
-  Expr.pattern_match arg p = some m →
-  Joinable cator (Expr.function ((p, body) :: f)) →
-  Joinable (Expr.app cator arg) (Expr.sub m body)
-:= by
-  unfold Joinable
-  intro h0 h1
-  have ⟨en,h2,h3⟩ := h1
-  clear h1
-  have h4 := NStepStar.function_inversion h3
-  rw [h4] at h2
-  clear h3 h4
-  exists (Expr.sub m body)
-  apply And.intro
-  { exact NStepStar.pattern_match h0 h2 }
-  { exact NStepStar.refl }
-
+-- theorem Joinable.pattern_match :
+--   Expr.pattern_match arg p = some m →
+--   Joinable cator (Expr.function ((p, body) :: f)) →
+--   Joinable (Expr.app cator arg) (Expr.sub m body)
+-- := by
+--   unfold Joinable
+--   intro h0 h1
+--   have ⟨en,h2,h3⟩ := h1
+--   clear h1
+--   have h4 := NStepStar.function_inversion h3
+--   rw [h4] at h2
+--   clear h3 h4
+--   exists (Expr.sub m body)
+--   apply And.intro
+--   { exact NStepStar.pattern_match h0 h2 }
+--   { exact NStepStar.refl }
 
 
 theorem NStepStar.skip :
@@ -645,118 +801,6 @@ theorem NRcdStepStar.joinable :
   apply And.intro h0 NRcdStepStar.refl
 
 
-mutual
-
-  theorem List.pattern_match_entry_subject_reduction :
-    NRcdStep r r' →
-    List.pattern_match_entry l p r = some m →
-    ∃ m' , List.pattern_match_entry l p r' = some m'
-  := by
-    intro h0 h1
-    cases h0 with
-    | @head l' r e e' fresh step =>
-      simp [List.pattern_match_entry] at h1
-      by_cases h3 : l' = l
-      {
-        simp [*] at h1
-        have ⟨m',ih⟩ := Expr.pattern_match_subject_reduction step h1
-        exists m'
-        simp [List.pattern_match_entry, *]
-      }
-      {
-        simp [*] at h1
-        exists m
-        simp [List.pattern_match_entry, *]
-      }
-
-    | @tail l' r r' e fresh step =>
-      simp [List.pattern_match_entry] at h1
-      by_cases h3 : l' = l
-      {
-        simp [*] at h1
-        exists m
-        simp [List.pattern_match_entry, *]
-
-      }
-      {
-        simp [*] at h1
-        have ⟨m',ih⟩ := List.pattern_match_entry_subject_reduction step h1
-        exists m'
-        simp [List.pattern_match_entry, *]
-      }
-
-
-
-  theorem List.pattern_match_record_subject_reduction :
-    NRcdStep r r' →
-    List.pattern_match_record r rp = some m →
-    ∃ m' , List.pattern_match_record r' rp = some m'
-  := by cases rp with
-  | nil =>
-    intro h0 h1
-    simp [List.pattern_match_record]
-  | cons lp rp' =>
-    have (l,p) := lp
-    intro h0 h1
-    simp [List.pattern_match_record] at h1
-    have ⟨h2,h3⟩ := h1
-    clear h1
-
-    cases h4 : (List.pattern_match_entry l p r) with
-    | some m0 =>
-      simp [h4] at h3
-      cases h5 : (List.pattern_match_record r rp') with
-      | some m1 =>
-        simp [h5] at h3
-        have ⟨h6,h7⟩ := h3
-        have ⟨m0',h8⟩ := List.pattern_match_entry_subject_reduction h0 h4
-        have ⟨m1',h9⟩ := List.pattern_match_record_subject_reduction h0 h5
-        exists (m0' ++ m1')
-        simp [List.pattern_match_record, *]
-
-      | none =>
-        simp [h5] at h3
-    | none =>
-      simp [h4] at h3
-
-
-  theorem Expr.pattern_match_subject_reduction :
-    NStep arg arg' →
-    Expr.pattern_match arg p = some m →
-    ∃ m' , Expr.pattern_match arg' p = some m'
-  := by cases p with
-  | var x =>
-    intro h0 h1
-    exists [(x,arg')]
-    simp [Expr.pattern_match]
-  | iso l p' =>
-    intro h0 h1
-    cases h0 with
-    | @iso e e' l' step =>
-      simp [Expr.pattern_match] at h1
-      have ⟨h2,h3⟩ := h1
-      clear h1
-      have ⟨m',ih⟩ := Expr.pattern_match_subject_reduction step h3
-      exists m'
-      simp [Expr.pattern_match]
-      exact ⟨h2, ih⟩
-    | _ =>
-      simp [Expr.pattern_match] at h1
-  | record ps =>
-    intro h0 h1
-    cases h0 with
-    | iso =>
-      simp [Expr.pattern_match] at h1
-    | @record r r' step =>
-      simp [Expr.pattern_match] at h1
-      have ⟨m',ih⟩ := List.pattern_match_record_subject_reduction step h1
-      exists m'
-      simp [Expr.pattern_match]
-      exact ih
-    | _ =>
-      simp [Expr.pattern_match] at h1
-end
-
 theorem Expr.sub_refl :
   x ∉ ListPair.dom m →
   (Expr.sub m (.var x)) = (.var x)
@@ -777,22 +821,6 @@ theorem Expr.sub_refl :
     unfold Expr.sub at ih
     exact ih
 
-
-theorem Expr.pattern_match_subject_star_reduction :
-  NStepStar arg arg' →
-  ∀ {m},
-  Expr.pattern_match arg p = some m →
-  ∃ m' , Expr.pattern_match arg' p = some m'
-:= by
-  intro h0
-  induction h0 with
-  | refl =>
-    intro m h1
-    exists m
-  | @step arg argm arg' h1 h2 ih =>
-    intro m h3
-    have ⟨m',h4⟩ := Expr.pattern_match_subject_reduction h1 h3
-    apply ih h4
 
 theorem NStep.sub_context_preservation
   m
@@ -987,29 +1015,6 @@ mutual
     | _ => simp [Expr.pattern_match] at matching_arg
 end
 
-theorem NStepStar.pattern_match_preservation :
-  NStepStar arg arg' →
-  ∀ {m m'},
-  Expr.pattern_match arg p = some m →
-  Expr.pattern_match arg' p = some m' →
-  ∀ body, NStepStar (Expr.sub m body) (Expr.sub m' body)
-:= by
-  intro h0
-  induction h0 with
-  | @refl arg =>
-    intro m m' h1 h2 body
-    rw [h1] at h2
-    simp at h2
-    rw [← h2]
-    apply NStepStar.refl
-  | @step arg argm arg' h1 h2 ih =>
-    intro m m' h3 h4 body
-    have ⟨mm,h5⟩ := Expr.pattern_match_subject_reduction h1 h3
-    have h6 := NStep.pattern_match_preservation h1 h3 h5 body
-    apply NStepStar.transitivity h6
-    apply ih h5
-    apply h4
-
 theorem Joinable.subject_star_expansion :
   NStepStar b b' →
   Joinable a b' →
@@ -1023,215 +1028,246 @@ theorem Joinable.subject_star_expansion :
   apply NStepStar.transitivity h0 h3
 
 
-mutual
-  theorem NRcdStep.semi_confluence
-    (step : NRcdStep r ra)
-    (step_star : NRcdStepStar r rb)
-  : RcdJoinable ra rb
-  := by
-  cases step with
-  | @head l r' e ea fresh step' =>
-    have ⟨eb,r'',h0,h1,h2⟩ := NRcdStepStar.cons_inversion step_star
-    rw [h0]
-    have joinable := NStep.semi_confluence step' h1
-    have rjoinable := NRcdStepStar.joinable h2
-    apply RcdJoinable.cons (Or.inl fresh) joinable rjoinable
 
-  | @tail l r ra' e fresh step' =>
-    have ⟨e',rb',h0,h1,h2⟩ := NRcdStepStar.cons_inversion step_star
-    rw [h0]
-    have joinable := NStepStar.joinable h1
-    have rjoinable := NRcdStep.semi_confluence step' h2
-    have h4 := List.is_fresh_key_nrcd_star_reduction h2 fresh
-    apply RcdJoinable.cons (Or.inr h4) joinable rjoinable
+-- mutual
+--   theorem NRcdStep.semi_confluence
+--     (step : NRcdStep r ra)
+--     (step_star : NRcdStepStar r rb)
+--   : RcdJoinable ra rb
+--   := by
+--   cases step with
+--   | @head l r' e ea fresh step' =>
+--     have ⟨eb,r'',h0,h1,h2⟩ := NRcdStepStar.cons_inversion step_star
+--     rw [h0]
+--     have joinable := NStep.semi_confluence step' h1
+--     have rjoinable := NRcdStepStar.joinable h2
+--     apply RcdJoinable.cons (Or.inl fresh) joinable rjoinable
 
-  theorem NStep.semi_confluence
-    (step : NStep e ea)
-    (step_star : NStepStar e eb)
-  : Joinable ea eb
-  := by cases step with
-  | @iso body body_a l step' =>
-    have ⟨body_b,h0,step_star'⟩ := NStepStar.iso_inversion step_star
-    rw [h0]
-    have ih := NStep.semi_confluence step' step_star'
-    exact Joinable.iso ih
-  | @record r ra step' =>
-    have ⟨rb,h0,step_star'⟩ := NStepStar.record_inversion step_star
-    rw [h0]
+--   | @tail l r ra' e fresh step' =>
+--     have ⟨e',rb',h0,h1,h2⟩ := NRcdStepStar.cons_inversion step_star
+--     rw [h0]
+--     have joinable := NStepStar.joinable h1
+--     have rjoinable := NRcdStep.semi_confluence step' h2
+--     have h4 := List.is_fresh_key_nrcd_star_reduction h2 fresh
+--     apply RcdJoinable.cons (Or.inr h4) joinable rjoinable
 
-    have ih := NRcdStep.semi_confluence step' step_star'
-    exact Joinable.record ih
-  | @applicator cator cator_a arg step' =>
-    cases NStepStar.app_inversion step_star with
-    | inl h0 =>
-      have ⟨cator_b,arg',h1,h2,h3⟩ := h0
-      rw [h1]
-      clear h0 h1 step_star
-      have joinable_cator := NStep.semi_confluence step' h2
-      have joinable_arg := NStepStar.joinable h3
-      exact Joinable.app joinable_cator joinable_arg
-    | inr h0 =>
-      cases h0 with
-      | inl h1 =>
-        have ⟨p,body,f,m,h2,h3,h4⟩ := h1
-        rw [h2]
-        clear h1 h2 step_star
-        have joinable_cator := NStep.semi_confluence step' h3
-        exact Joinable.pattern_match h4 joinable_cator
+--   theorem NStep.semi_confluence
+--     (step : NStep e ea)
+--     (step_star : NStepStar e eb)
+--   : Joinable ea eb
+--   := by cases step with
+--   | @iso body body_a l step' =>
+--     have ⟨body_b,h0,step_star'⟩ := NStepStar.iso_inversion step_star
+--     rw [h0]
+--     have ih := NStep.semi_confluence step' step_star'
+--     exact Joinable.iso ih
+--   | @record r ra step' =>
+--     have ⟨rb,h0,step_star'⟩ := NStepStar.record_inversion step_star
+--     rw [h0]
 
-      | inr h1 =>
-        have ⟨isval, p, body, f,h2,h3,h4⟩ := h1
-        rw [h2]
-        clear h1 h2 step_star
-        have joinable_cator := NStep.semi_confluence step' h3
-        exact Joinable.skip isval h4 joinable_cator
+--     have ih := NRcdStep.semi_confluence step' step_star'
+--     exact Joinable.record ih
+--   | @applicator cator cator_a arg step' =>
 
-  | @applicand arg arg_a cator step' =>
-    cases NStepStar.app_inversion step_star with
-    | inl h0 =>
-      have ⟨cator',arg_b,h1,h2,h3⟩ := h0
-      clear h0
-      rw [h1]
-      clear h1 step_star
-      have joinable_cator := NStepStar.joinable h2
-      have joinable_arg := NStep.semi_confluence step' h3
-      exact Joinable.app joinable_cator joinable_arg
-    | inr h0 =>
-      cases h0 with
-      | inl h1 =>
-        have ⟨p,body,f,m,h2,h3,h4⟩ := h1
-        rw [h2]
-        clear h1 h2 step_star
-        have ⟨m',h5⟩ := Expr.pattern_match_subject_reduction step' h4
-        have h6 := NStep.pattern_match_preservation step' h4 h5 body
-        apply Joinable.subject_star_expansion h6
-        have joinable_cator := NStepStar.joinable h3
-        exact Joinable.pattern_match h5 joinable_cator
-
-      | inr h1 =>
-        have ⟨isval, p, body, f,h2,h3,h4⟩ := h1
-        have h5 := NStep.not_value step' isval
-        exact False.elim h5
-
-  | @pattern_match arg p m body f matching =>
-    cases NStepStar.app_inversion step_star with
-    | inl h0 =>
-      have ⟨cator,arg',h1,h2,h3⟩ := h0
-      rw [h1]
-      clear step_star h0 h1
-      have h4 := NStepStar.function_inversion h2
-      rw [h4]
-      clear h2 h4
-
-      have ⟨m',h5⟩ := Expr.pattern_match_subject_star_reduction h3 matching
-      have h6 := NStepStar.pattern_match_preservation h3 matching h5 body
-      apply Joinable.swap
-      apply Joinable.subject_star_expansion h6
-      apply Joinable.pattern_match h5
-      apply Joinable.refl
-
-    | inr h0 =>
-      cases h0 with
-      | inl h1 =>
-        have ⟨p',body',f',m',h2,h3,h4⟩ := h1
-        rw [h2]
-        clear step_star h1 h2
-        have h5 := NStepStar.function_inversion h3
-        simp at h5
-        have ⟨⟨h6,h7⟩,h8⟩ := h5
-        clear h5
-        rw [h7]
-        clear h7
-        rw [h6] at h4
-        clear h6 h8
-        rw [matching] at h4
-        simp at h4
-        rw [← h4]
-        apply Joinable.refl
-
-      | inr h1 =>
-        have ⟨isval,p',body',f',h2,h3,h4⟩ := h1
-        rw [h2]
-        clear step_star h1 h2
-        have h5 := NStepStar.function_inversion h3
-        simp at h5
-        have ⟨⟨h6,h7⟩,h8⟩ := h5
-        clear h5
-        rw [h6] at h4
-        simp [matching] at h4
-
-  | @skip arg p body f isval h0 =>
-    cases NStepStar.app_inversion step_star with
-    | inl h1 =>
-      have ⟨cator,arg',h2,h3,h4⟩ := h1
-      rw [h2]
-      clear step_star h1 h2
-      apply NStepStar.value_inversion isval at h4
-      rw [h4]
-      clear h4
-      have h5 := NStepStar.function_inversion h3
-      rw [h5]
-      clear h5
-      apply Joinable.swap
-      apply Joinable.skip isval h0
-      apply Joinable.refl
-    | inr h1 =>
-      cases h1 with
-      | inl h2 =>
-        have ⟨p',body',f',m,h3,h4,h5⟩ := h2
-        rw [h3]
-        clear step_star h2 h3
-
-        have h6 := NStepStar.function_inversion h4
-        simp at h6
-        have ⟨⟨h7,h8⟩,h9⟩ := h6
-        clear h4 h6
-        rw [h8]
-        rw [h7] at h5
-        rw [h0] at h5
-        simp at h5
-
-      | inr h2 =>
-        have ⟨isval',p',body',f',h3,h4,h5⟩ := h2
-        rw [h3]
-        clear step_star h2 h3
-        have h6 := NStepStar.function_inversion h4
-        simp at h6
-        have ⟨⟨h7,h8⟩,h9⟩ := h6
-        rw [h9]
-        apply Joinable.refl
-
-  -- | @loopi body body' step=>
-
-    -- have ⟨body_b,h0,step_star'⟩ := NStepStar.loop_inversion step_star
-    -- rw [h0]
-    -- have ih := NStep.semi_confluence step' step_star'
-    -- exact Joinable.iso ih
-    -- sorry
-  | _ => sorry
-end
+--     cases NStepStar.app_inversion step_star with
+--     | inl h0 =>
+--       have ⟨cator_b,arg',h1,h2,h3⟩ := h0
+--       rw [h1]
+--       clear h0 h1 step_star
+--       have joinable_cator := NStep.semi_confluence step' h2
+--       have joinable_arg := NStepStar.joinable h3
+--       exact Joinable.app joinable_cator joinable_arg
+--     | inr h0 =>
+--       cases h0 with
+--       | inl h1 =>
+--         have ⟨m',body,p,f,arg',h2,h3,h4,h5⟩ := h1
+--         clear h1
+--         have joinable_cator := NStep.semi_confluence step' h3
 
 
+--         -- have joinable_arg := NStepStar.joinable h4
+--         -- have joinable_app := Joinable.app joinable_cator joinable_arg
+
+--       ----------------------------
+
+--         -- have ⟨m,h6⟩ := Expr.pattern_match_subject_star_expansion h4 h5
+
+--         -- have h7 := NStepStar.pattern_match_preservation h4 h6 h5 body
+--         -- apply Joinable.subject_star_reduction h7
+--         -- exact Joinable.pattern_match h6 joinable_cator
+
+--       | inr h1 =>
+--         have ⟨isval, p, body, f,h2,h3,h4⟩ := h1
+--         rw [h2]
+--         clear h1 h2 step_star
+--         have joinable_cator := NStep.semi_confluence step' h3
+--         exact Joinable.skip isval h4 joinable_cator
+
+--   | @applicand arg arg_a cator step' =>
+--     cases NStepStar.app_inversion step_star with
+--     | inl h0 =>
+--       have ⟨cator',arg_b,h1,h2,h3⟩ := h0
+--       clear h0
+--       rw [h1]
+--       clear h1 step_star
+--       have joinable_cator := NStepStar.joinable h2
+--       have joinable_arg := NStep.semi_confluence step' h3
+--       exact Joinable.app joinable_cator joinable_arg
+--     | inr h0 =>
+--       cases h0 with
+--       | inl h1 =>
+--         have ⟨m',body,p,f,arg',h2,h3,h4,h5⟩ := h1
+--         rw [h2]
+--         clear h1 h2 step_star
+--         /- TODO: figure out how to use new inversion definition -/
+--         -- have ⟨m',h5⟩ := Expr.pattern_match_subject_reduction step' h4
+--         -- have h6 := NStep.pattern_match_preservation step' h4 h5 body
+--         -- apply Joinable.subject_star_expansion h6
+--         -- have joinable_cator := NStepStar.joinable h3
+--         -- exact Joinable.pattern_match h5 joinable_cator
+
+--       | inr h1 =>
+--         have ⟨isval, p, body, f,h2,h3,h4⟩ := h1
+--         have h5 := NStep.not_value step' isval
+--         exact False.elim h5
+
+--   | @pattern_match arg p m body f matching =>
+--     cases NStepStar.app_inversion step_star with
+--     | inl h0 =>
+--       have ⟨cator,arg',h1,h2,h3⟩ := h0
+--       rw [h1]
+--       clear step_star h0 h1
+--       have h4 := NStepStar.function_inversion h2
+--       rw [h4]
+--       clear h2 h4
+
+--       /- TODO -/
+--       -- have ⟨m',h5⟩ := Expr.pattern_match_subject_star_reduction h3 matching
+--       -- have h6 := NStepStar.pattern_match_preservation h3 matching h5 body
+--       -- apply Joinable.swap
+--       -- apply Joinable.subject_star_expansion h6
+--       -- apply Joinable.pattern_match h5
+--       -- apply Joinable.refl
+
+--     | inr h0 =>
+--       cases h0 with
+--       | inl h1 =>
+--         have ⟨p',body',f',m',h2,h3,h4⟩ := h1
+--         rw [h2]
+--         clear step_star h1 h2
+--         have h5 := NStepStar.function_inversion h3
+--         simp at h5
+--         have ⟨⟨h6,h7⟩,h8⟩ := h5
+--         clear h5
+--         rw [h7]
+--         clear h7
+--         rw [h6] at h4
+--         clear h6 h8
+--         rw [matching] at h4
+--         simp at h4
+--         rw [← h4]
+--         apply Joinable.refl
+
+--       | inr h1 =>
+--         have ⟨isval,p',body',f',h2,h3,h4⟩ := h1
+--         rw [h2]
+--         clear step_star h1 h2
+--         have h5 := NStepStar.function_inversion h3
+--         simp at h5
+--         have ⟨⟨h6,h7⟩,h8⟩ := h5
+--         clear h5
+--         rw [h6] at h4
+--         simp [matching] at h4
+
+--   | @skip arg p body f isval h0 =>
+--     cases NStepStar.app_inversion step_star with
+--     | inl h1 =>
+--       have ⟨cator,arg',h2,h3,h4⟩ := h1
+--       rw [h2]
+--       clear step_star h1 h2
+--       apply NStepStar.value_inversion isval at h4
+--       rw [h4]
+--       clear h4
+--       have h5 := NStepStar.function_inversion h3
+--       rw [h5]
+--       clear h5
+--       apply Joinable.swap
+--       apply Joinable.skip isval h0
+--       apply Joinable.refl
+--     | inr h1 =>
+--       cases h1 with
+--       | inl h2 =>
+--         have ⟨p',body',f',m,h3,h4,h5⟩ := h2
+--         rw [h3]
+--         clear step_star h2 h3
+
+--         have h6 := NStepStar.function_inversion h4
+--         simp at h6
+--         have ⟨⟨h7,h8⟩,h9⟩ := h6
+--         clear h4 h6
+--         rw [h8]
+--         rw [h7] at h5
+--         rw [h0] at h5
+--         simp at h5
+
+--       | inr h2 =>
+--         have ⟨isval',p',body',f',h3,h4,h5⟩ := h2
+--         rw [h3]
+--         clear step_star h2 h3
+--         have h6 := NStepStar.function_inversion h4
+--         simp at h6
+--         have ⟨⟨h7,h8⟩,h9⟩ := h6
+--         rw [h9]
+--         apply Joinable.refl
+
+--   -- | @loopi body body' step=>
+
+--     -- have ⟨body_b,h0,step_star'⟩ := NStepStar.loop_inversion step_star
+--     -- rw [h0]
+--     -- have ih := NStep.semi_confluence step' step_star'
+--     -- exact Joinable.iso ih
+--     -- sorry
+--   | _ => sorry
+-- end
+
+
+-- theorem NStepStar.confluence :
+--   NStepStar e a →
+--   NStepStar e b →
+--   Joinable a b
+-- := by
+--   intro h0 h1
+--   apply NStepStar.reverse at h0
+--   induction h0 with
+--   | refl =>
+--     unfold Joinable
+--     exists b
+--     apply And.intro h1 .refl
+--   | @step m a h2 h3 ih =>
+--     have ⟨b',h4,h5⟩ := ih
+--     clear ih
+--     have ⟨n,h6,h7⟩ := NStep.semi_confluence h3 h4
+--     exists n
+--     apply And.intro h6
+--     apply NStepStar.transitivity h5 h7
+
+
+/- TODO: define parallel step
+  - prove diamond property
+  - induct on parallel step
+-/
 theorem NStepStar.confluence :
   NStepStar e a →
   NStepStar e b →
   Joinable a b
-:= by
-  intro h0 h1
-  apply NStepStar.reverse at h0
-  induction h0 with
-  | refl =>
-    unfold Joinable
-    exists b
-    apply And.intro h1 .refl
-  | @step m a h2 h3 ih =>
-    have ⟨b',h4,h5⟩ := ih
-    clear ih
-    have ⟨n,h6,h7⟩ := NStep.semi_confluence h3 h4
-    exists n
-    apply And.intro h6
-    apply NStepStar.transitivity h5 h7
+:= by sorry
 
+
+theorem NStepStar.semi_confluence :
+  NStep e a →
+  NStepStar e b →
+  Joinable a b
+:= by sorry
 
 
 theorem NStep.local_confluence :
@@ -1240,7 +1276,7 @@ theorem NStep.local_confluence :
   Joinable a b
 := by
   intro h0 h1
-  apply NStep.semi_confluence
+  apply NStepStar.semi_confluence
   { exact h0 }
   { apply NStepStar.step h1 NStepStar.refl }
 
