dsn/Lang/Dynamic/ParStep.lean
@@ -1,0 +1,156 @@
+import Lang.Util
+import Lang.Basic
+import Lang.Dynamic.NStep
+
+set_option pp.fieldNotation false
+
+namespace Lang.Dynamic
+
+mutual
+
+  inductive ParRcdStep : List (String × Expr) → List (String × Expr) → Prop
+  | cons :
+    List.is_fresh_key l r → ParStep e e' →  NRcdStep r r' →
+    ParRcdStep ((l, e) :: r) ((l, e') :: r)
+
+  inductive ParStep : Expr → Expr → Prop
+  | refl e : ParStep e e
+  /- head normal forms -/
+  | iso : ParStep body body' → ParStep (.iso l body) (.iso l body')
+  | record : ParRcdStep r r' →  ParStep (.record r) (.record r')
+
+  /- redex forms -/
+  | app arg :
+    ParStep cator cator' → ParStep arg arg' →
+    ParStep (.app cator arg) (.app cator' arg)
+  | pattern_match body f :
+    Expr.pattern_match arg p = some m →
+    ParStep (.app (.function ((p,body) :: f)) arg) (Expr.sub m body)
+  | skip body f:
+    arg.is_value →
+    Expr.pattern_match arg p = none →
+    ParStep (.app (.function ((p,body) :: f)) arg) (.app (.function f) arg)
+  | erase body t :
+    ParStep (.anno body t) body
+  | loopi : ParStep body body' → ParStep (.loop body) (.loop body')
+  | recycle x e :
+    ParStep
+      (.loop (.function [(.var x, e)]))
+      (Expr.sub [(x, (.loop (.function [(.var x, e)])))] e)
+end
+
+
+def Joinable (R : α → α → Prop) (ea eb : α) :=
+  ∃ en , R ea en ∧ R eb en
+
+mutual
+
+  theorem ParStep.diamond
+    (step_a : ParStep e ea)
+    (step_b : ParStep e eb)
+  : Joinable ParStep ea eb
+  := by cases step_a with
+  | refl =>
+    exists eb
+    apply And.intro step_b
+    exact ParStep.refl eb
+  | _ => sorry
+
+end
+
+
+theorem ReflTrans.par_step_soundness :
+  ReflTrans ParStep e e' → ReflTrans NStep e e'
+:= by sorry
+
+
+theorem ReflTrans.par_step_completeness :
+  ReflTrans NStep e e' → ReflTrans ParStep e e'
+:= by sorry
+
+theorem Joinable.right_par_step_expansion :
+  ParStep e e' →
+  Joinable (ReflTrans ParStep) ea e' →
+  Joinable (ReflTrans ParStep) ea e
+:= by
+  unfold Joinable
+  intro h0 h1
+  have ⟨en,h2,h3⟩ := h1
+  clear h1
+  exists en
+  apply And.intro
+  { exact h2 }
+  { exact ReflTrans.step h0 h3 }
+
+theorem ReflTrans.par_step_semi_confluence
+  (step : ReflTrans ParStep e ea)
+: ∀ {eb} , ParStep e eb → Joinable (ReflTrans ParStep) ea eb
+:= by induction step with
+| refl e =>
+  intro eb h0
+  unfold Joinable
+  exists eb
+  apply And.intro
+  { apply ReflTrans.step
+    { exact h0 }
+    { exact ReflTrans.refl eb }
+  }
+  { exact ReflTrans.refl eb }
+| @step e em ea h0 h1 ih =>
+  intro eb h2
+  have h3 := ParStep.diamond h0 h2
+  unfold Joinable at h3
+  have ⟨en,h4,h5⟩ := h3
+  clear h3
+  specialize ih h4
+  exact Joinable.right_par_step_expansion h5 ih
+
+theorem ReflTrans.par_step_confluence
+  (step_a : ReflTrans ParStep e ea)
+  (step_b : ReflTrans ParStep e eb)
+: Joinable (ReflTrans ParStep) ea eb
+:= by
+  have h0 := ReflTrans.reverse step_a
+  clear step_a
+  induction h0 with
+  | refl =>
+    unfold Joinable
+    exists eb
+    apply And.intro
+    { apply step_b }
+    { exact ReflTrans.refl eb }
+  | @step m a h2 h3 ih =>
+    have ⟨b',h4,h5⟩ := ih
+    clear ih
+    have ⟨n,h6,h7⟩ := ReflTrans.par_step_semi_confluence h4 h3
+    exists n
+    apply And.intro
+    { exact h7 }
+    { exact ReflTrans.transitivity h5 h6 }
+
+theorem Joinable.par_step_soundness :
+  Joinable (ReflTrans ParStep) ea eb →
+  Joinable (ReflTrans NStep) ea eb
+:= by
+  unfold Joinable
+  intro h0
+  have ⟨en,h1,h2⟩ := h0 ; clear h0
+  exists en
+  apply And.intro
+  { exact ReflTrans.par_step_soundness h1 }
+  { exact ReflTrans.par_step_soundness h2 }
+
+
+theorem ReflTrans.n_step_confluence
+  (step_a : ReflTrans NStep e ea)
+  (step_b : ReflTrans NStep e eb)
+: Joinable (ReflTrans NStep) ea eb
+:= by
+  apply Joinable.par_step_soundness
+  apply ReflTrans.par_step_confluence
+  { exact ReflTrans.par_step_completeness step_a }
+  { exact ReflTrans.par_step_completeness step_b }
+
+
+
+end Lang.Dynamic
